wip on Linearizability

raft/Linearizability.v
@@ -37,6 +37,9 @@ Section Linearizability.
   Definition acknowledged_op (k : K) (trace : list op) :=
     In (O k) trace.
 
+  Definition acknowledged_op_dec (k : K) (tr : list op) : {acknowledged_op k tr} + {~acknowledged_op k tr} :=
+    in_dec op_eq_dec (O k) tr.
+
   Inductive acknowledge_all_ops : list op ->  list IR -> Prop :=
   | AAO_nil : acknowledge_all_ops [] []
   | AAO_IU : forall k tr out,
@@ -55,22 +58,184 @@ Section Linearizability.
               acknowledge_all_ops tr out ->
               acknowledge_all_ops (O k :: tr) (IRO k :: out).
 
+  Lemma acknowledge_all_ops_was_in :
+    forall l ir,
+      acknowledge_all_ops l ir ->
+      forall k,
+        In (IRI k) ir ->
+        In (I k) l.
+  Proof.
+    induction 1; intros; simpl in *; intuition (auto; congruence).
+  Qed.
+
+  Fixpoint acknowledge_all_ops_func (l : list op) (target : list IR) : list IR :=
+    match l with
+      | [] => []
+      | x :: xs => let tr := acknowledge_all_ops_func xs target in
+                   match x with
+                     | I k => if acknowledged_op_dec k xs
+                              then IRI k :: tr
+                              else if in_dec IR_eq_dec (IRU k) target
+                                   then IRI k :: IRU k :: tr
+                                   else tr
+                     | O k => IRO k :: tr
+                   end
+    end.
+
+  Hint Constructors acknowledge_all_ops.
+
+  Lemma acknowledge_all_ops_func_correct :
+    forall l target,
+      acknowledge_all_ops l (acknowledge_all_ops_func l target).
+  Proof.
+    induction l; intros; simpl; repeat break_match; subst; eauto.
+  Qed.
+
+  Lemma acknowledge_all_ops_func_target_ext :
+    forall l t t',
+      (forall k, In (IRU k) t -> In (IRU k) t') ->
+      (forall k, In (IRU k) t' -> In (IRU k) t) ->
+      acknowledge_all_ops_func l t = acknowledge_all_ops_func l t'.
+  Proof.
+    induction l; simpl in *; repeat break_match; subst; intuition eauto using f_equal.
+    repeat break_match; eauto using f_equal; solve [exfalso; eauto].
+  Qed.
+
   Definition good_move (x y : IR) : Prop :=
-    (forall k k', x <> IRO k /\ y <> IRI k').
+    (forall k k', ~ (x = IRO k /\ y = IRI k')) /\
+    (forall k, ~ (x = IRI k /\ y = IRO k)) /\
+    (forall k, ~ (x = IRI k /\ y = IRU k)).
 
   Inductive IR_equivalent : list IR -> list IR -> Prop :=
-  | equiv_nil : IR_equivalent [] []
-  | equiv_cons : forall x xs ys,
+  | IR_equiv_nil : IR_equivalent [] []
+  | IR_equiv_cons : forall x xs ys,
                    IR_equivalent xs ys ->
                    IR_equivalent (x :: xs) (x :: ys)
-  | equiv_move : forall x y xs ys,
+  | IR_equiv_move : forall x y xs ys,
                    IR_equivalent xs ys ->
                    good_move x y ->
                    IR_equivalent (x :: y :: xs) (y :: x :: ys)
-  | equiv_trans : forall l1 l2 l3,
+  | IR_equiv_trans : forall l1 l2 l3,
                     IR_equivalent l1 l2 ->
                     IR_equivalent l2 l3 ->
                     IR_equivalent l1 l3.
+  Hint Constructors IR_equivalent.
+
+  Lemma IR_equivalent_refl :
+    forall l,
+      IR_equivalent l l.
+  Proof.
+    induction l; eauto.
+  Qed.
+
+  Lemma IR_equiv_in_l_r :
+    forall ir1 ir2,
+      IR_equivalent ir1 ir2 ->
+      forall o,
+        In o ir1 -> In o ir2.
+  Proof.
+    induction 1; intros; simpl in *; intuition.
+  Qed.
+
+  Lemma IR_equiv_in_r_l :
+    forall ir1 ir2,
+      IR_equivalent ir1 ir2 ->
+      forall o,
+        In o ir2 -> In o ir1.
+  Proof.
+    induction 1; intros; simpl in *; intuition.
+  Qed.
+
+  Require Import Permutation.
+  Hint Constructors Permutation.
+  Lemma IR_equiv_Permutation :
+    forall ir1 ir2,
+      IR_equivalent ir1 ir2 ->
+      Permutation ir1 ir2.
+  Proof.
+    induction 1; eauto.
+  Qed.
+
+  Lemma IR_equiv_app_head :
+    forall l xs ys,
+      IR_equivalent xs ys ->
+      IR_equivalent (l ++ xs) (l ++ ys).
+  Proof.
+    induction l; intros; simpl; auto.
+  Qed.
+
+  Lemma IR_equiv_snoc :
+    forall xs ys x,
+      IR_equivalent xs ys ->
+      IR_equivalent (xs ++ [x]) (ys ++ [x]).
+  Proof.
+    induction 1; simpl; eauto.
+  Qed.
+
+  Lemma IR_equiv_app_tail :
+    forall l xs ys,
+      IR_equivalent xs ys ->
+      IR_equivalent (xs ++ l) (ys ++ l).
+  Proof.
+    induction 1; intros; simpl in *; eauto using IR_equivalent_refl.
+  Qed.
+
+  Section Examples.
+    Example IR_equiv_eg1 :
+      forall k k',
+        k <> k' ->
+        IR_equivalent [IRI k; IRI k'; IRO k; IRO k'] [IRI k; IRO k; IRI k'; IRO k'].
+    Proof.
+      intros.
+      constructor.
+      econstructor; auto.
+      red.
+      intuition (auto; congruence).
+    Qed.
+
+    Example IR_equiv_eg2 :
+      forall k k',
+        k <> k' ->
+        IR_equivalent [IRI k; IRI k'; IRO k; IRO k'] [IRI k'; IRO k'; IRI k; IRO k].
+    Proof.
+      intros.
+      eapply IR_equiv_trans with (l2 := [IRI k; IRI k'; IRO k'; IRO k]).
+      - repeat constructor; unfold good_move; intuition (try congruence).
+      - eapply IR_equiv_trans with (l2 := [IRI k'; IRI k; IRO k'; IRO k]).
+        + apply IR_equiv_move; auto using IR_equivalent_refl.
+          red. intuition congruence.
+        + constructor. apply IR_equiv_move; auto.
+          red. intuition congruence.
+    Qed.
+
+    Example IR_equiv_eg3 :
+      forall k k',
+        k <> k' ->
+        IR_equivalent [IRI k; IRI k'; IRO k'; IRO k] [IRI k'; IRO k'; IRI k; IRO k].
+    Proof.
+      intros.
+      eapply IR_equiv_trans with (l2 := [IRI k'; IRI k; IRO k'; IRO k]).
+      - constructor.
+        + apply IR_equivalent_refl.
+        + red. intuition congruence.
+      - constructor. constructor.
+        + apply IR_equivalent_refl.
+        + red. intuition congruence.
+    Qed.
+
+    Example IR_equiv_eg4 :
+      forall k k',
+        k <> k' ->
+        IR_equivalent [IRI k; IRI k'; IRO k'; IRO k] [IRI k; IRO k; IRI k'; IRO k'].
+    Proof.
+      intros.
+      constructor.
+      eapply IR_equiv_trans with (l2 := [IRI k'; IRO k; IRO k']).
+      - repeat constructor; unfold good_move; intuition congruence.
+      - eapply IR_equiv_move; auto.
+        red. intuition congruence.
+    Qed.
+  End Examples.
 
   Fixpoint good_trace (l : list IR) : Prop :=
     match l with
@@ -81,23 +246,445 @@ Section Linearizability.
     end.
 
   Definition equivalent (l : list op) (ir : list IR) : Prop :=
+    good_trace ir /\
     exists ir',
       acknowledge_all_ops l ir' /\
-      IR_equivalent ir' ir /\
-      good_trace ir.
+      IR_equivalent ir' ir.
 
-  Functional Scheme good_trace_ind := Induction for  good_trace Sort Prop.
+  Lemma acknowledge_all_ops_func_IRU_In :
+    forall l ir k,
+      In (IRU k) (acknowledge_all_ops_func l ir) ->
+      In (I k) l.
+  Proof.
+    induction l; intros; simpl in *; repeat break_match; subst; simpl in *;
+    intuition (eauto; congruence).
+  Qed.
+
+  Definition get_op_input_keys (l : list op) : list K :=
+    filterMap (fun x => match x with
+                          | I k => Some k
+                          | _ => None
+                        end) l.
+
+  Definition get_IR_input_keys (l : list IR) : list K :=
+    filterMap (fun x => match x with
+                          | IRI k => Some k
+                          | _ => None
+                        end) l.
+
+  Lemma get_IR_input_keys_defn :
+    forall x l,
+      get_IR_input_keys (x :: l) = match x with
+                               | IRI k => k :: get_IR_input_keys l
+                               | _ => get_IR_input_keys l
+                             end.
+  Proof.
+    unfold get_IR_input_keys.
+    intros.
+    simpl. repeat break_match; congruence.
+  Qed.
+
+  (* this is cleaner than the auto-generated functional induction scheme *)
+  Fixpoint good_trace_ind'
+    (P : list IR -> Prop -> Prop)
+    (l : list IR) :
+      P [] True ->
+      (forall k, P [IRI k] False) ->
+      (forall k k' l, P (IRI k :: IRI k' :: l) False) ->
+      (forall k k' l, P l (good_trace l) -> P (IRI k :: IRO k' :: l) (k = k' /\ good_trace l)) ->
+      (forall k k' l, P l (good_trace l) -> P (IRI k :: IRU k' :: l) (k = k' /\ good_trace l)) ->
+      (forall k l, P (IRO k :: l) False) ->
+      (forall k l, P (IRU k :: l) False) ->
+      P l (good_trace l).
+  Proof.
+    intros.
+    destruct l; simpl; repeat break_match; auto; subst.
+    - apply H2. apply good_trace_ind'; auto.
+    - apply H3. apply good_trace_ind'; auto.
+  Qed.
+
+  Lemma good_trace_ind :
+    forall P : list IR -> Prop -> Prop,
+      P [] True ->
+      (forall k, P [IRI k] False) ->
+      (forall k k' ir, P (IRI k :: IRI k' :: ir) False) ->
+      (forall k k' ir, P ir (good_trace ir) -> P (IRI k :: IRO k' :: ir) (k = k' /\ good_trace ir)) ->
+      (forall k k' ir, P ir (good_trace ir) -> P (IRI k :: IRU k' :: ir) (k = k' /\ good_trace ir)) ->
+      (forall k ir, P (IRO k :: ir) False) ->
+      (forall k ir, P (IRU k :: ir) False) ->
+      forall ir, P ir (good_trace ir).
+  Proof.
+    intros.
+    apply good_trace_ind'; auto.
+  Qed.
+
+  Lemma good_trace_IRI_in :
+    forall ir,
+      good_trace ir ->
+      forall k,
+        In (IRI k) ir ->
+        In (IRO k) ir \/ In (IRU k) ir.
+  Proof.
+    intros ir.
+    induction ir, good_trace using good_trace_ind; intros; simpl in *; intuition (auto; try congruence).
+    - subst. find_apply_hyp_hyp. intuition.
+    - subst. find_apply_hyp_hyp. intuition.
+  Qed.
+
+  Lemma acknowledge_all_ops_func_target_nil :
+    forall l,
+      (forall k, ~ In (O k) l) ->
+      acknowledge_all_ops_func l [] = [].
+  Proof.
+    induction l; intros; simpl in *.
+    - auto.
+    - repeat break_match; subst; unfold acknowledged_op in *;
+      (exfalso + idtac); solve [intuition eauto].
+  Qed.
+
+  Lemma before_In :
+    forall A x y l,
+      before (A:=A) x y l ->
+      In x l.
+  Proof.
+    induction l; intros; simpl in *; intuition.
+  Qed.
+
+  Lemma before_head_op :
+    forall l h ir,
+      (forall k1 k2,
+         In (I k2) l ->
+         before (O k1) (I k2) l ->
+         before (IRO k1) (IRI k2) (IRI h :: ir)) ->
+      forall x,
+        In (I h) l ->
+        before x (I h) l ->
+        exists k,
+          x = I k.
+  Proof.
+    intros. destruct x. eauto.
+    eapply H in H1; auto.
+    simpl in *. intuition congruence.
+  Qed.
+
+  Lemma before_split :
+    forall A l (x y : A),
+      before x y l ->
+      x <> y ->
+      In x l ->
+      In y l ->
+      exists xs ys zs,
+        l = xs ++ x :: ys ++ y :: zs.
+  Proof.
+    induction l; intros; simpl in *; intuition; subst; try congruence.
+    - exists nil. simpl. find_apply_lem_hyp in_split. break_exists. subst. eauto.
+    - exists nil. simpl. find_apply_lem_hyp in_split. break_exists. subst. eauto.
+    - eapply_prop_hyp In In; eauto. break_exists. subst.
+      exists (a :: x0), x1, x2. auto.
+  Qed.
+
+  Lemma In_app_before :
+    forall A xs ys x y
+           (A_eq_dec : forall a b : A, {a=b} + {a<>b}),
+      In(A:=A) x xs ->
+      (~ In y xs) ->
+      before x y (xs ++ y :: ys).
+  Proof.
+    induction xs; intros; simpl in *; intuition.
+    destruct (A_eq_dec a x); intuition.
+  Qed.
+
+  Lemma good_move_II :
+    forall k k',
+      good_move (IRI k) (IRI k').
+  Proof.
+    red. intuition congruence.
+  Qed.
+
+  Lemma good_move_OO :
+    forall k k',
+      good_move (IRO k) (IRO k').
+  Proof.
+    red. intuition congruence.
+  Qed.
+
+  Lemma IR_equivalent_all_Is :
+    forall l k,
+      (forall x, In x l -> exists k, x = IRI k) ->
+      IR_equivalent (l ++ [IRI k]) (IRI k :: l).
+  Proof.
+    induction l; intros; simpl in *; intuition.
+    apply IR_equiv_trans with (l2 := (a :: IRI k :: l)).
+    - auto.
+    - specialize (H a). concludes. break_exists. subst.
+      auto using IR_equivalent_refl, good_move_II.
+  Qed.
+
+  Definition good_op_move (x y : op) : Prop :=
+    (forall k k', ~ (x = O k /\ y = I k')) /\
+    (forall k, ~ (x = I k /\ y = O k)).
+
+  Inductive op_equivalent : list op -> list op -> Prop :=
+  | op_equiv_nil : op_equivalent [] []
+  | op_equiv_cons : forall x xs ys, op_equivalent xs ys -> op_equivalent (x :: xs) (x :: ys)
+  | op_equiv_move : forall x y xs ys, good_op_move x y ->
+                                      op_equivalent xs ys -> op_equivalent (x :: y :: xs) (y :: x :: ys)
+  | op_equiv_trans : forall l1 l2 l3, op_equivalent l1 l2 -> op_equivalent l2 l3 -> op_equivalent l1 l3.
+
+  Lemma op_equiv_Permutation :
+    forall xs ys,
+      op_equivalent xs ys ->
+      Permutation xs ys.
+  Proof.
+    induction 1; eauto.
+  Qed.
+
+  Lemma op_equiv_ack_op_lr :
+    forall xs ys,
+      op_equivalent xs ys ->
+      forall k,
+        acknowledged_op k xs ->
+        acknowledged_op k ys.
+  Proof.
+    unfold acknowledged_op.
+    intros.
+    eauto using Permutation_in, op_equiv_Permutation.
+  Qed.
+
+  Lemma op_equiv_ack_op_rl :
+    forall xs ys,
+      op_equivalent xs ys ->
+      forall k,
+        acknowledged_op k ys ->
+        acknowledged_op k xs.
+  Proof.
+    unfold acknowledged_op.
+    intros.
+    eauto using Permutation_sym, Permutation_in, op_equiv_Permutation.
+  Qed.
+
+  Lemma acknowledged_op_defn :
+    forall k xs,
+      acknowledged_op k xs ->
+      In (O k) xs.
+  Proof.
+    auto.
+  Qed.
+
+  Lemma good_move_U_l :
+    forall k x,
+      good_move (IRU k) x.
+  Proof.
+    red. intuition congruence.
+  Qed.
+
+  Lemma good_move_IU_neq :
+    forall k k',
+      k <> k' ->
+      good_move (IRI k) (IRU k').
+  Proof.
+    red. intuition congruence.
+  Qed.
+
+  Lemma good_move_IO_neq :
+    forall k k',
+      k <> k' ->
+      good_move (IRI k) (IRO k').
+  Proof.
+    red. intuition congruence.
+  Qed.
+
+  Hint Resolve IR_equivalent_refl.
+  Hint Resolve good_move_II.
+  Hint Resolve good_move_U_l.
+
+  Lemma not_good_op_move_IO :
+    forall k,
+      good_op_move (I k) (O k) -> False.
+  Proof.
+    unfold good_op_move.
+    intuition eauto.
+  Qed.
+
+  Lemma not_good_op_move_OI :
+    forall k k',
+      good_op_move (O k) (I k') -> False.
+  Proof.
+    unfold good_op_move.
+    intuition eauto.
+  Qed.
+
+  Lemma good_op_move_good_move_IO :
+    forall k k',
+      good_op_move (I k) (O k') ->
+      good_move (IRI k) (IRO k').
+  Proof.
+    unfold good_op_move, good_move.
+    intuition (try congruence). repeat find_inversion. eauto.
+  Qed.
+
+  Lemma op_equiv_AAOF_IR_equiv :
+    forall xs ys,
+      op_equivalent xs ys ->
+      forall l,
+        IR_equivalent (acknowledge_all_ops_func xs l) (acknowledge_all_ops_func ys l).
+  Proof.
+    induction 1; intros.
+    - auto.
+    - simpl.
+      repeat break_match; subst; auto;
+      exfalso; eauto using op_equiv_ack_op_lr, op_equiv_ack_op_rl.
+    - simpl.
+      repeat break_match; subst; intuition; try congruence;
+      try solve [exfalso; eauto using op_equiv_ack_op_lr, op_equiv_ack_op_rl];
+      auto;
+      try solve [exfalso; eauto using Permutation_in, op_equiv_Permutation, acknowledged_op_defn, Permutation_sym];
+      try solve [repeat find_inversion; exfalso; eauto using not_good_op_move_IO, not_good_op_move_OI].
+      + eapply IR_equiv_trans; [apply IR_equiv_move; auto|]. constructor.
+        eapply IR_equiv_trans; [apply IR_equiv_move; auto|]; auto.
+        apply good_move_IU_neq.
+        intro; subst;
+        exfalso; eauto using Permutation_in, op_equiv_Permutation, acknowledged_op_defn.
+      + auto using good_op_move_good_move_IO.
+      + eauto.
+      + destruct (K_eq_dec k k0).
+        * subst. auto.
+        * eapply IR_equiv_trans; [apply IR_equiv_cons; apply IR_equiv_move; auto|].
+          eapply IR_equiv_trans; [apply IR_equiv_move; auto|]. constructor.
+          eapply IR_equiv_trans; [apply IR_equiv_cons; apply IR_equiv_move; auto|].
+          auto using good_move_IU_neq.
+      + eapply IR_equiv_trans; [apply IR_equiv_cons; apply IR_equiv_move; auto|].
+        eapply IR_equiv_trans; [apply IR_equiv_move; auto|]. apply good_move_IO_neq. congruence.
+        auto.
+      + auto using good_move_OO.
+    - eauto.
+  Qed.
+
+  Hint Constructors op_equivalent.
+
+  Lemma op_equivalent_refl :
+    forall xs,
+      op_equivalent xs xs.
+  Proof.
+    induction xs; auto.
+  Qed.
+
+  Lemma good_op_move_II :
+    forall k k',
+      good_op_move (I k) (I k').
+  Proof.
+    red. intuition congruence.
+  Qed.
+
+  Lemma op_equivalent_all_Is :
+    forall l k,
+      (forall x, In x l -> exists k, x = I k) ->
+      op_equivalent (l ++ [I k]) (I k :: l).
+  Proof.
+    induction l; intros; simpl in *; intuition.
+    apply op_equiv_trans with (l2 := (a :: I k :: l)).
+    - auto.
+    - specialize (H a). concludes. break_exists. subst.
+      auto using op_equivalent_refl, good_op_move_II.
+  Qed.
+
+  Lemma op_equiv_app_tail :
+    forall l xs ys,
+      op_equivalent xs ys ->
+      op_equivalent (xs ++ l) (ys ++ l).
+  Proof.
+    induction 1; intros; simpl in *; intuition.
+    - auto using op_equivalent_refl.
+    - eauto.
+  Qed.
+
+  Lemma IR_equivalent_acknowledge_all_ops_func :
+    forall ir,
+      good_trace ir ->
+      forall l,
+      (forall k, In (O k) l -> In (IRO k) ir) ->
+      (forall k, In (IRO k) ir -> In (O k) l) ->
+      (forall k, In (IRU k) ir -> In (I k) l) ->
+      (forall k k', In (I k') l ->
+                    before (O k) (I k') l ->
+                    before (IRO k) (IRI k') ir) ->
+      (forall k, In (O k) l -> before (I k) (O k) l) ->
+      (forall k, In (IRI k) ir -> In (I k) l) ->
+      NoDup (get_op_input_keys l) ->
+      NoDup (get_IR_input_keys ir) ->
+      IR_equivalent (acknowledge_all_ops_func l ir) ir.
+  Proof.
+    intros ir.
+    induction ir, good_trace using good_trace_ind; intros; try solve [simpl in *; intuition].
+    - rewrite acknowledge_all_ops_func_target_nil; auto.
+    - match goal with
+        | [ H : good_trace (_ :: _) |- _ ] => simpl in H
+      end.
+      break_and. subst.
+      assert (In (O k') l) by firstorder.
+      assert (In (I k') l) by eauto using before_In.
+      assert (before (I k') (O k') l) by auto.
+      repeat rewrite get_IR_input_keys_defn in *.
+      match goal with
+        | [ H : NoDup (_ :: _) |- _ ] => invc H
+      end.
+
+      assert (forall x, before x (I k') l -> exists k, x = I k) by eauto using before_head_op.
+
+      find_copy_apply_lem_hyp before_split; auto; try congruence. break_exists. subst.
+
+      eapply IR_equiv_trans.
+      + apply op_equiv_AAOF_IR_equiv.
+        rewrite app_comm_cons.
+        rewrite <- app_ass.
+        apply op_equiv_app_tail.
+        replace (x ++ I k' :: x0) with ((x ++ [I k']) ++ x0) by now rewrite app_ass.
+        apply op_equiv_app_tail.
+        apply op_equivalent_all_Is.
+        intros.
+        apply H7. apply In_app_before; auto using op_eq_dec. admit. (* from NoDup stuff... *)
+      + repeat rewrite app_ass. rewrite <- app_comm_cons.
+        unfold acknowledge_all_ops_func. fold acknowledge_all_ops_func.
+        break_if.
+        * constructor.
+          admit.
+        (* continue from here: pull the O out to the front and cancel
+           using lemma similar to all_Is. then because k' can not
+           appear in rest of l, get rid of first two elements of
+           target and recurse. *)
+        * { break_if.
+            - admit. (* contradiction: need NoDup on outputs *)
+            - exfalso. apply n. red. intuition.
+          }
+    - (* IRU case. *)
+  Admitted.
 
   Theorem equivalent_intro :
     forall l ir,
       good_trace ir ->
       (forall k, In (O k) l -> In (IRO k) ir) ->
       (forall k, In (IRO k) ir -> In (O k) l) ->
-      (forall k k', In (I k') l -> before (O k) (I k') l ->
-               before (IRO k) (IRI k') ir) ->
+      (forall k, In (IRU k) ir -> In (O k) l) ->
+      (forall k k', In (I k') l ->
+                    before (O k) (I k') l ->
+                    before (IRO k) (IRI k') ir) ->
+      (forall k, In (O k) l -> before (I k) (O k) l) ->
+      NoDup (get_op_input_keys l) ->
+      NoDup (get_IR_input_keys ir) ->
       equivalent l ir.
   Proof.
-  Admitted.
+    intros.
+    red.
+    intuition.
+    exists (acknowledge_all_ops_func l ir).
+    intuition.
+    - apply acknowledge_all_ops_func_correct.
+    - apply IR_equivalent_acknowledge_all_ops_func; auto.
+      firstorder using good_trace_IRI_in, before_In.
+      intros.
+      find_apply_lem_hyp good_trace_IRI_in; auto.
+      intuition eauto using before_In.
+  Qed.
 
 (*
   Lemma good_trace_acknowledge_all_ops_id :
@@ -115,15 +702,6 @@ Section Linearizability.
       apply AAO_IO.
       + constructor. auto.
       + apply AAO_O. auto.
-  Qed.
-
-  Lemma IR_equivalent_refl :
-    forall l,
-      IR_equivalent l l.
-  Proof.
-    induction l.
-    - constructor.
-    - constructor. auto.
   Qed.
 
   Lemma good_trace_equiv :
